Modularize our map implementation

KeyManagement/ChMaps.v
@@ -1,29 +1,20 @@
 From Coq Require Import
-     FSets.FMapList
-     FSets.FMapFacts
      Structures.OrderedType
      Structures.OrderedTypeEx
-     Logic.ProofIrrelevance
-     Program.Equality
 .
 
-Require Import MyPrelude Tactics.
+Require Import MyPrelude Tactics Maps.
 
 Inductive channel_id := 
 | Single (n : nat)
 | Intersection (ch1 ch2 : nat)
 .
 
-Module ChannelType <: OrderedType.
+Module ChannelType <: UsualOrderedType.
   Definition t := channel_id.
 
-  Definition eq ch1 ch2 :=
-    match (ch1, ch2) with
-    | (Single n, Single n') => n = n'
-    | (Intersection n1 n2, Intersection n1' n2') => n1 = n1' /\ n2 = n2'
-    | _ => False
-    end.
-
+  Definition eq := @eq t.
+    
   Definition lt ch1 ch2 : Prop :=
     match (ch1, ch2) with
     | (Single n, Single n') => n < n'
@@ -32,30 +23,9 @@ Module ChannelType <: OrderedType.
     | (Single _, Intersection _ _) => False
     end.
 
-  Lemma eq_refl :
-    forall x, eq x x.
-  Proof.
-    intros; unfold eq; destruct x; eauto.
-  Qed.
-  
-  Lemma eq_sym :
-    forall x y, eq x y -> eq y x.
-  Proof.
-    unfold eq; intros; destruct x, y; eauto.
-    invert H. eauto.
-  Qed.
-
-  Lemma eq_trans :
-    forall x y z, eq x y -> eq y z -> eq x z.
-  Proof.
-    unfold eq; intros; destruct x, y, z;
-    repeat (match goal with
-    | [ H1 : ?n1 = ?n2, H2 : ?n2 = ?n3 |- ?n1 = ?n3 ] => rewrite H1; rewrite H2; trivial
-    | [ H : False |- _ ] => inversion H
-    | [ H : _ /\ _ |- _ ] => split_ands
-    | [ |- _ = _ /\ _ = _ ] => split
-    end).
-  Qed.
+  Definition eq_refl := @eq_refl t.
+  Definition eq_sym := @eq_sym t.
+  Definition eq_trans := @eq_trans t.
 
   Lemma lt_trans :
     forall x y z, lt x y -> lt y z -> lt x z.
@@ -67,41 +37,44 @@ Module ChannelType <: OrderedType.
   Lemma lt_not_eq :
     forall x y, lt x y -> ~ eq x y.
   Proof.
-    intros; destruct x, y. unfold lt in H. unfold eq. Nat.order.
-    unfold eq. eauto. unfold eq; eauto. unfold lt, eq in *.
-    split_ands; split_ors; subst; unfold not; intros; split_ands;
-      Nat.order.
+    intros * H; destruct x, y; unfold lt in H; unfold not, eq;
+      intro EQ; invert EQ; split_ors; subst; try Nat.order.
   Qed.
 
   Lemma compare :
     forall( x y : t), Compare lt eq x y.
   Proof.
-    intros.  destruct x, y. 
-    case_eq (Nat.compare n n0); intro. 
-    apply EQ. now apply nat_compare_eq.
-    apply LT. now apply nat_compare_lt.
-    apply GT. now apply nat_compare_gt.
-    apply GT. unfold lt. eauto.
-    apply LT. unfold lt. eauto.
-    case_eq (Nat.compare ch1 ch0); intro.
-    case_eq (Nat.compare ch2 ch3); intro.
-    apply EQ. unfold eq. split; now apply nat_compare_eq.
-    apply LT. unfold lt. left. split. now apply nat_compare_eq.
-    now apply nat_compare_lt.
-    apply GT. left. split. apply Nat.eq_sym. now apply nat_compare_eq. now apply nat_compare_gt.
+    intros.
+    destruct x, y.
+    case_eq (Nat.compare n n0); intro.
+    apply EQ; unfold eq; f_equal; now apply nat_compare_eq.
+    apply LT; unfold lt; now apply nat_compare_lt.
+    apply GT; unfold lt; now apply nat_compare_gt.
+    apply GT; unfold lt; eauto.
+    apply LT; unfold lt; eauto.
+    case_eq (Nat.compare ch1 ch0).
+    case_eq (Nat.compare ch2 ch3); intros.
+    apply EQ. unfold eq; f_equal; now apply nat_compare_eq.
+    apply LT; unfold lt; f_equal; left.
+    split; [ now apply nat_compare_eq
+           | now apply nat_compare_lt].
+    apply GT; unfold lt; left. split. apply Nat.eq_sym. now apply nat_compare_eq. now apply nat_compare_gt.
 
-    apply LT. unfold lt. right. now apply nat_compare_lt.
-    apply GT. unfold lt. right. now apply nat_compare_gt.
+    intros; apply LT. unfold lt. right. now apply nat_compare_lt.
+    intros; apply GT. unfold lt. right. now apply nat_compare_gt.
   Defined.
 
   Lemma eq_dec :
     forall x y, { eq x y } + { ~ eq x y }.
   Proof.
-    unfold eq; destruct x, y; try tauto.
-    eapply eq_nat_dec.
+    unfold eq; destruct x, y.
+    - destruct (eq_dec n n0); subst; eauto.
+      right; intros H; invert H; contradiction.
+    - right; unfold not; intros; discriminate.
+    - right; unfold not; intros; discriminate.
 
-    cases (ch1 ==n ch0); cases (ch2 ==n ch3); cases (ch1 ==n ch3); cases (ch2 ==n ch0); subst;
-      eauto; right; unfold not; intros; split_ors; contradiction.
+    - cases (ch1 ==n ch0); cases (ch2 ==n ch3); cases (ch1 ==n ch3); cases (ch2 ==n ch0); subst;
+        eauto; right; unfold not; intros H; invert H; contradiction.
   Qed.
 
 End ChannelType.
@@ -114,643 +87,14 @@ Definition combine (ch1 ch2 : channel_id) :=
   | _ => None
   end.
 
-Module Import ChMap := FMapList.Make(ChannelType).
-Module P := WProperties_fun ChannelType ChMap.
-Module F := P.F.
-Module O := OrdProperties ChMap.
+Module Import ChMap := MyOrderedMap( ChannelType ).
 
-Export ChMap P F O.
-
-From Coq Require List.
-
-Set Implicit Argruments.
-
-Module ChNotation.
+Module ChMapNotation.
   Notation "#0" := (empty _).
   Notation "m #+ ( k , v )" := (add k v m) (at level 50, left associativity).
   Notation "m #- k" := (remove k m) (at level 50, left associativity).
   Notation "m #? k" := (find k m) (at level 50, left associativity).
-End ChNotation.
+End ChMapNotation.
 
-Import ChNotation.
+Export ChMapNotation.
   
-Module Import OTF := OrderedType.OrderedTypeFacts ChannelType.
-Module Import OMF := FSets.FMapFacts.OrdProperties ChMap.
-
-Lemma lookup_empty_none :
-  forall {A} k,
-    (@empty A) #? k = None.
-Proof. unfold find, Raw.find; trivial. Qed.
-
-Ltac context_map_rewrites1 :=
-  match goal with
-  | [ H : ?m #? ?k = _ |- context[?m #? ?k] ] => rewrite H
-  | [ H1 : context [match ?m with _ => _ end],
-           H2 : ?m = _ |- _ ] => rewrite H2 in H1
-  end.
-
-Ltac contra_map_lookup1 :=
-  match goal with
-  | [ H : ?chs #? ?ch = ?v -> _, ARG : ?chs #? ?ch = ?v |- _ ] => specialize (H ARG)
-  | [ H1 : ?chs #? ?ch = _, H2 : ?chs #? ?ch = _ |- _ ] => rewrite H1 in H2; invert H2
-  | [ H : ?chs #? ?ch = _ |- context [ ?chs #? ?ch <> _ ] ] => unfold not; intros
-  end.
-
-(* rewrite all of these with idtac, see where they fail then come back and uncomment the failures;
-   the remaining idtac lines never get called, try changing by whatever for rewrites *)
-Ltac clean_map_lookups1 :=
-  invert_base_equalities1
-  || contra_map_lookup1
-  || context_map_rewrites1
-  || match goal with
-    | [ H : context [ #0 #? _ ] |- _ ] =>
-      idtac
-    (* rewrite lookup_empty_none in H *)
-    | [ H : _ #? (?ch,_) #? ?ch = _ |- _ ] =>
-      rewrite add_eq_o in H by trivial
-    | [ H : _ #+ (?ch1,_) #? ?ch2 = _ |- _ ] =>
-      rewrite add_neq_o in H by auto 2
-    | [ H : _ #+ (?ch1,_) #? ?ch2 = _ |- _ ] =>
-      rewrite add_eq_o in H by auto 2
-    | [ H : _ #? (?ch,_) #? ?ch = _ |- _ ] =>
-      rewrite add_eq_o in H by trivial
-    | [ H : _ #+ (?ch1,_) #? ?ch2 = _ |- _ ] =>
-      rewrite add_neq_o in H by auto 2
-    | [ H : _ #+ (?ch1,_) #? ?ch2 = _ |- _ ] =>
-      rewrite add_eq_o in H by auto 2
-    | [ H : context [ match _ #+ (?ch,_) #? ?ch with _ => _ end ] |- _ ] => rewrite add_eq_o in H by trivial
-    | [ H : context [ match _ #+ (?ch1,_) #? ?ch2 with _ => _ end ] |- _ ] => rewrite add_neq_o in H by auto 2
-    | [ H : context [ match _ #+ (?ch1,_) #? ?ch2 with _ => _ end ] |- _ ] => rewrite add_eq_o in H by auto 2
-    | [ |- context[_ #+ (?ch,_) #? ?ch] ] => rewrite add_eq_o by trivial
-    | [ |- context[_ #+ (?ch1,_) #? ?ch2] ] => rewrite add_neq_o by auto 2
-    | [ |- context[_ #+ (?ch1,_) #? ?ch2] ] => rewrite add_eq_o by auto 2
-    | [ |- context[_ #- ?ch #? ?ch] ] => rewrite remove_eq_o by trivial
-    | [ |- context[_ #- ?ch1 #? ?ch2] ] => rewrite remove_neq_o by auto 2
-    | [ |- context[_ #- ?ch1 #? ?ch2] ] => rewrite remove_eq_o by auto 2
-    | [ H : ~ In _ _ |- _ ] => rewrite not_find_in_iff in H
-    | [ |- ~ In _ _ ] => rewrite not_find_in_iff
-    | [ H : In _ _ |- _ ] => rewrite in_find_iff in H
-    | [ H1 : ?m #? ?ch = _ , H2 : ?m #? ?ch = _ |- _] => rewrite H1 in H2
-    | [ H1 : ?m #? ?ch1 = _ , H2 : ?m #? ?ch2 = _ |- _] => assert (ch1 = ch2) as RW by auto 2; rewrite RW in H1; clear RW; rewrite H1 in H2
-    | [ H : ?m #? ?ch <> None |- _ ] => cases (m #? ch); try contradiction; clear H
-    | [ H : MapsTo _ _ _ |- _ ] => rewrite find_mapsto_iff in H
-    | [ |- context [ MapsTo _ _ _ ] ] => rewrite find_mapsto_iff
-    | [ |- ~False ] => tauto
-    | [ H : False |- _] => tauto
-    | [ _ : not (?ch1 = ?ch0 /\ ?ch2 = ?ch3) |- not (?ch0 = ?ch1 /\ ?ch3 = ?ch2) ] => unfold not; intro; split_ands; subst; eauto
-    end
-.
-
-Ltac contra_chmap_lookup := repeat (invert_base_equalities1 || contra_map_lookup1).
-Ltac clean_chmap_lookups := repeat clean_map_lookups1.
-Ltac context_chmap_rewrites := repeat context_map_rewrites1.
-
-Section MapLemmas.
-
-  (* Lemma reversed_rewrite : *)
-  (*   forall ch1 ch2, *)
-  (*     ChannelType.eq (Intersection ch1 ch2) (Intersection ch2 ch1). *)
-  (* Proof. *)
-  (*   intros. unfold ChannelType.eq; right; split; reflexivity. *)
-  (* Qed. *)
-
-  (* Does not work since List.In relies on = not eq *)
-  Lemma lookup_some_implies_in :
-    forall V (m : ChMap.t V) ch v,
-      m #? ch = Some v
-      -> List.In (ch, v) (to_list m).
-  Proof.
-    intros * H. rewrite <- find_mapsto_iff, elements_mapsto_iff, InA_alt in H.
-    unfold to_list. split_ex.
-    unfold eq_key_elt in H.  unfold Raw.PX.eqke in H. simpl in H; split_ands; subst.
-
-    destruct ch, x, k; split_ex; simpl in *.
-    rewrite H. assumption. invert H. invert H. split_ands; rewrite H, H1; assumption.
-  Qed.
-  
-
-  Ltac reorder_intersection_neq :=
-    match goal with
-    | [ n : ~ (?ch1 = ?ch0 /\ ?ch2 = ?ch3) |- ~ ChannelType.eq (Intersection ?ch0 ?ch3) (Intersection ?ch1 ?ch2) ] => 
-      unfold ChannelType.eq; unfold not; intro; split_ands
-    (* | [ h : not (?ch0 = ?ch1 /\ ?ch2 = ?ch3) |- not ChannelType.eq (Intersection ch0 ch2) (Intersection ch1 ch3) ] => *)
-    (*   unfold ChannelType.eq; unfold not; intro; split_ands *)
-    (* | [ H : ~ (?ch1 = ?ch0 /\ ?ch2 = ?ch3) |- ~ ChannelType.eq (Intersection ch0 ch3) (Intersection ch1 ch2) ] => *)
-    (*   unfold ChannelType.eq; unfold not; intro; split_and *)
-    end; eauto. 
-
-  Lemma lookup_split :
-    forall V (m : ChMap.t V) k k' v v',
-      (m #+ (k, v)) #? k' = Some v'
-      -> (~(ChannelType.eq k' k) /\ m #? k' = Some v') \/ ((ChannelType.eq k' k) /\ v' = v).
-  Proof.
-    intros.
-    cases (eq_dec k k'); intros; subst; clean_chmap_lookups.
-    destruct k, k'; invert y; eauto.
-    destruct k, k'; left; split; eauto. reorder_intersection_neq.
-  Qed.
-
-  Lemma map_eq_fields_eq :
-    forall {V} (th th' : Raw.t V) s s',
-        th = th'
-      -> {| this := th ; sorted := s |} = {| this := th' ; sorted := s' |}.
-  Proof.
-    intros; subst; f_equal; apply proof_irrelevance.
-  Qed.
-
-  Lemma map_eq_elements_eq :
-    forall {V} (m m' : ChMap.t V),
-      elements m = elements m'
-      -> m = m'.
-  Proof.
-    intros. destruct m, m'.
-    simpl in *. eapply map_eq_fields_eq; eauto.
-  Qed.
-
-  Lemma lt_contra :
-    forall x y, ChannelType.lt x y -> ChannelType.lt y x -> False.
-  Proof.
-    intros. destruct x, y; unfold ChannelType.lt in *. Nat.order. invert H. invert H0.
-    split_ands; split_ors; try Nat.order.
-  Qed.
-  
-  Lemma Equal_hd_tl :
-    forall {V} (m1 m1' m2 m2' : t V) x xs y ys sx sy,
-        m1 = {| this := x  :: xs ; sorted := sx |}
-      -> m2 = {| this := y :: ys ; sorted := sy |}
-      -> Equal m1 m2
-      -> m1' = m1 #- fst x
-      -> m2' = m2 #- fst y
-      -> x = y /\ Equal m1' m2'.
-  Proof.
-    intros.
-
-    destruct x as [n1 v1]; destruct y as [n2 v2]; simpl in *.
-
-    assert ( (n1,v1) = (n2,v2) ).
-    - unfold Equal in *; subst; simpl in *.
-      match goal with
-      | [ H : forall _, _ |- _ ] =>
-        generalize (H n1); generalize (H n2); intros
-      end;
-        unfold find, Raw.find in *; simpl in *.
-      
-      pose proof (Raw.MX.elim_compare_eq (ChannelType.eq_refl n1)) as EQn1.
-      pose proof (Raw.MX.elim_compare_eq (ChannelType.eq_refl n2)) as EQn2.
-      split_ex.
-      rewrite H2, H3 in *.
-
-      cases (ChannelType.compare n1 n2);
-        cases (ChannelType.compare n2 n1);
-        try discriminate; subst; repeat invert_base_equalities1; eauto;
-          repeat
-            match goal with
-            | [ H : ChannelType.eq _ _ |- _ ] => unfold ChannelType.eq in H; subst
-            end; eauto.
-      destruct n1, n2. rewrite e. trivial. invert e. invert e. split_ands. rewrite e0. rewrite e6. trivial.
-      destruct n1, n2. rewrite e. trivial. invert e. invert e. split_ands. rewrite e. rewrite e4. trivial.
-      destruct n1, n2. rewrite e. trivial. invert e. invert e. split_ands. rewrite e. rewrite e4. trivial.
-      clear Heq. eapply lt_contra in l. invert l. assumption.
-      
-    - split; auto; subst.
-
-      pose proof (Raw.MX.elim_compare_eq (ChannelType.eq_refl n2)); split_ex.
-      unfold Equal in *; simpl in *.
-
-      intro k; invert H4. destruct n2, k.
-      * case (n ==n n0); intros; subst; (rewrite !remove_eq_o by auto 2) || (rewrite !remove_neq_o by auto 2); eauto.
-      * assert (not (ChannelType.eq (Single n) (Intersection ch1 ch2))). unfold ChannelType.eq; eauto.
-        (rewrite !remove_neq_o by auto 2); eauto.
-      * assert (not (ChannelType.eq (Single n) (Intersection ch1 ch2))). unfold ChannelType.eq; eauto.
-        (rewrite !remove_neq_o by auto 2); eauto.
-      * cases (ch1 ==n ch0); cases (ch2 ==n ch3).
-      + rewrite !remove_eq_o by auto 2; trivial.
-      + assert (not (ChannelType.eq (Intersection ch1 ch2) (Intersection ch0 ch3))); unfold ChannelType.eq, not. intro. split_ands. tauto.
-        rewrite !remove_neq_o by auto 2; eauto.
-      + assert (not (ChannelType.eq (Intersection ch1 ch2) (Intersection ch0 ch3))); unfold ChannelType.eq, not. intro. split_ands. tauto.
-        rewrite !remove_neq_o by auto 2; eauto.
-      + assert (not (ChannelType.eq (Intersection ch1 ch2) (Intersection ch0 ch3))); unfold ChannelType.eq, not. intro. split_ands. tauto.
-        rewrite !remove_neq_o by auto 2; eauto.
-  Qed.
-
-  Lemma remove_hd :
-    forall {V} n (v : V) xs sx hdrel,
-      {| this := (n,v) :: xs ; sorted := Sorted.Sorted_cons sx hdrel |} #- n = {| this := xs ; sorted := sx |}.
-  Proof.
-    intros. unfold remove. eapply map_eq_elements_eq; simpl.
-    pose proof (Raw.MX.elim_compare_eq (ChannelType.eq_refl n)); split_ex.
-    rewrite H; trivial.
-  Qed.
-
-  Lemma Empty_eq_empty :
-    forall v m,
-      Empty (elt:=v) m
-      -> #0 = m.
-  Proof.
-    intros. apply elements_Empty in H. apply map_eq_elements_eq. auto.
-  Qed.
-
-  Lemma map_eq_Equal :
-    forall {V} (m m' : t V),
-      Equal m m'
-      -> m = m'.
-  Proof.
-    destruct m as [l sl].
-    generalize dependent l.
-    induction l; intros.
-
-    - unfold Equal in H. simpl in *.
-      apply map_eq_elements_eq; simpl.
-      symmetry in H.
-
-      destruct m'; simpl in *.
-      cases this0; trivial.
-      exfalso.
-      destruct p; specialize (H c).
-      unfold find, Raw.find in *; simpl in *.
-        
-      pose proof (Raw.MX.elim_compare_eq (ChannelType.eq_refl c)); split_ex.
-      rewrite H0 in H.
-      discriminate.
-
-    - simpl.
-      destruct m'; cases this0; simpl in *.
-      + destruct a as [n v].
-        unfold Equal in H; specialize (H n).
-        unfold find, Raw.find in H; simpl in H.
-        pose proof (Raw.MX.elim_compare_eq) as P; specialize (P n n (ChannelType.eq_refl n)); destruct P.
-        rewrite H0 in H; discriminate.
-
-      + eapply Equal_hd_tl in H; eauto; split_ands; subst.
-        unfold Equal in H0; simpl in *.
-        dependent destruction sl.
-        dependent destruction sorted0.
-        specialize (IHl sl {| this := this0 ; sorted := sorted0 |}).
-
-        assert (tlEQ : Equal {| this := l ; sorted := sl |} {| this := this0 ; sorted := sorted0 |} ).
-        * destruct p;
-            unfold Equal; intro k;
-              specialize (H0 k); rewrite !remove_hd in H0; eauto.
-        * specialize (IHl tlEQ).
-          dependent destruction IHl.
-          eapply map_eq_elements_eq; simpl; f_equal.
-  Qed.
-
-  Lemma empty_Empty :
-    forall {V}, Empty (elt:=V) #0.
-  Proof.
-    intros.
-    unfold Empty, Raw.Empty, Raw.PX.MapsTo, not; intros.
-    invert H.
-  Qed.
-
-  Ltac _o_handle_single :=
-    match goal with
-    | [ |- context[_ #+ (Single ?n, _) #? Single ?n0]] => destruct (n ==n n0); subst; clean_chmap_lookups
-    end.
-
-  Lemma map_add_eq :
-    forall {V} (m : ChMap.t V) k v1 v2,
-      m #+ (k,v1) #+ (k,v2) = m #+ (k,v2).
-  Proof.
-    intros; apply map_eq_Equal; unfold Equal; intros. 
-    destruct (eq_dec k y); subst; clean_chmap_lookups; eauto.
-  Qed.
-
-  Lemma map_add_remove_eq :
-    forall {V} (m : ChMap.t V) k v1,
-      m #+ (k, v1) #- k = m #- k.
-  Proof.
-    intros; apply map_eq_Equal; unfold Equal; intros. 
-    destruct (eq_dec k y); subst; clean_chmap_lookups; eauto.
-  Qed.
-
-  Lemma map_add_remove_neq :
-    forall {V} (m : ChMap.t V) k1 v1 k2,
-        k1 <> k2
-      -> m #+ (k1, v1) #- k2 = m #- k2 #+ (k1, v1).
-  Proof.
-    intros. apply map_eq_Equal; unfold Equal; intros.
-
-    destruct (eq_dec k2 y); destruct (eq_dec k1 y); intros; subst; clean_chmap_lookups; eauto.
-    destruct y, k1, k2; subst; eauto; split_ands; subst; try contradiction.
-  Qed.
-
-  Lemma map_ne_swap :
-    forall {V} (m : ChMap.t V) k1 v1 k2 v2,
-      k1 <> k2
-      -> m #+ (k1,v1) #+ (k2,v2) = m #+ (k2,v2) #+ (k1,v1).
-  Proof.
-    intros.
-    apply map_eq_Equal; unfold Equal; intros.
-    destruct (eq_dec k2 y); destruct (eq_dec k1 y); intros; subst; clean_chmap_lookups; eauto.
-    destruct y, k1, k2; subst; eauto; split_ands; subst; try contradiction.
-  Qed.
-
-  Lemma map_remove_not_in_idempotent :
-    forall {V} (m : ChMap.t V) k1,
-      m #? k1 = None
-      -> m #- k1 = m.
-  Proof.
-    intros.
-    eapply map_eq_Equal; unfold Equal; intros.
-    
-    destruct (eq_dec y k1); subst; clean_chmap_lookups; eauto;
-    destruct y, k1; subst; eauto; clean_chmap_lookups; auto.
-    subst; eauto. rewrite remove_neq_o by clean_chmap_lookups. reflexivity.
-  Qed.
-
-End MapLemmas.
-
-Ltac Equal_eq :=
-  repeat
-    match goal with
-    | [ H : Equal _ _ |- _] => apply map_eq_Equal in H; subst
-    end.
-
-Ltac m_equal :=
-  repeat match goal with
-         (* | [ |- context[find ?k (add ?k' _ _) ] ] => idtac k; idtac k'; case (eq_dec k k'); intro *)
-         | [ |- context[find ?k (add ?k _ _) ] ]  => idtac
-           (* rewrite add_eq_o by (simple apply @eq_refl) *)
-         | [ |- context[find ?k (add ?k' _ _) ] ] => idtac
-           (* rewrite add_neq_o by ( (unfold not; intros ?SIMPLEQ; invert SIMPLEQ) || intuition idtac ) *)
-         (* | [ |- (add _ _ _) = _ ] => normalize_set *)
-         | [ |- (add _ _ _) = _ ] => unfold add, Raw.add; simpl
-         | [ |- {| this := _ ; sorted := _ |} = _ ] => eapply map_eq_fields_eq
-         | [ H : ?m #? ?k = None |- None = ?m #? ?k ] => eapply Empty_eq_empty; exact H
-         | [ H : None = ?m #? ?k |- ?m #? ?k = None ] => eapply Empty_eq_empty; exact H
-         | [ H : Empty ?m |- #0 = ?m ] => eapply Empty_eq_empty; exact H
-         | [ H : Empty ?m |- ?m = #0 ] => symmetry
-         | [ |- empty _ = _ ] => unfold empty, Raw.empty, remove, Raw.remove; simpl
-         end.
-
-Lemma remove_not_in_map_idempotent :
-  forall V (m : ChMap.t V) k,
-    m #? k = None
-    -> m #- k = m.
-Proof.
-  intros; apply map_eq_Equal; unfold Equal; intros;
-  destruct (eq_dec k y); subst; context_chmap_rewrites; clean_chmap_lookups; trivial.
-  destruct k, y; split_ands; subst; eauto; try contradiction.
-Qed.
-
-Ltac solve_simple_maps1 :=
-  clean_map_lookups1
-  || match goal with
-    | [ |- context [ _ #+ (?k1,_) #? ?k2 ] ] => destruct (eq_dec k1 k2); subst
-    | [ H : context [ _ #+ (?k1,_) #? ?k2 ] |- _ ] => destruct (eq_dec k1 k2); subst
-    | [ |- context [ match ?m #? ?k with _ => _ end ]] => cases (m #? k)
-    | [ H : context [ match ?m #? ?k with _ => _ end ] |- _ ] => cases (m #? k)
-    | [ |- context [ ?m #+ (?k,_) #+ (?k,_) ]] => rewrite map_add_eq by trivial
-    (* maybe a little too specific? *)
-    | [ |- context [ ?m #+ (?k1,_) #+ (?k2,_) = ?m #+ (?k2,_) #+ (?k1,_)]] => rewrite map_ne_swap by auto 2; trivial
-    end.
-
-Ltac solve_simple_maps := repeat solve_simple_maps1.
-
-Ltac maps_equal1 :=
-  match goal with
-  | [ |- _ #+ (_,_) = _ ] => apply map_eq_Equal; unfold Equal; intros
-  | [ |- _ = _ #+ (_,_) ] => apply map_eq_Equal; unfold Equal; intros
-  end
-  || solve_simple_maps1.
-
-(* TODO -- think of how to eliminate this *)
-Ltac maps_equal :=
-  apply map_eq_Equal; unfold Equal; intros;
-  (repeat solve_simple_maps1); trivial.
-
-Ltac canonicalize_map m :=
-  match m with
-  | context [ add ?k ?v ?m1 ] =>
-    match m1 with
-    | context [ add k _ _ ] =>
-      assert ( CANON : m = m #- k #+ (k,v) ); [
-        maps_equal
-      | repeat
-          (rewrite map_add_remove_eq in CANON by trivial)
-        || (rewrite map_add_remove_neq in CANON by eauto)
-        || (rewrite remove_not_in_map_idempotent in CANON by eauto)
-      ]; rewrite !CANON;
-      match type of CANON with
-      | _ = ?m' => clear CANON; try canonicalize_map m'
-      end
-    end
-  end.
-
-Lemma canonicalize_map_test1 :
-  forall V (m : ChMap.t V) k1 k2 (v1 v2 v3 : V),
-    k1 <> k2
-    -> m #? k1 = None
-    -> m #+ (k1,v1) #+ (k2,v2) #+ (k1,v3) = m #+ (k2,v2) #+ (k1,v3).
-Proof.
-  intros.
-  match goal with
-  | [ |- ?m = _ ] => canonicalize_map m
-  end; maps_equal.
-Qed.
-
-(* Lemma canonicalize_map_test2 : *)
-(*   forall V (m : ChMap.t V) k1 k2 k3 (v1 v2 v3 v4 : V), *)
-(*     k1 <> k2 *)
-(*     -> k1 <> k3 *)
-(*     -> k2 <> k3 *)
-(*     -> m #? k1 = None *)
-(*     -> m #+ (k1,v1) #+ (k2,v2) #+ (k1,v3) #+ (k3,v4) = m #+ (k2,v2) #+ (k1,v3) #+ (k3,v4). *)
-(* Proof. *)
-(*   intros. *)
-(*   match goal with *)
-(*   | [ |- ?m = _ ] => canonicalize_map m *)
-(*   end; maps_equal. *)
-(* Qed. *)
-
-(* Lemma canonicalize_map_test3 : *)
-(*   forall V (m : NatMap.t V) k1 k2 k3 (v1 v2 v3 v4 : V), *)
-(*     k1 <> k2 *)
-(*     -> k1 <> k3 *)
-(*     -> k2 <> k3 *)
-(*     -> m #? k1 = None *)
-(*     -> m #+ (k1,v1) #+ (k2,v2) #+ (k1,v3) #+ (k2,v4) #+ (k3,v4) = m #+ (k2,v4) #+ (k1,v3) #+ (k3,v4). *)
-(* Proof. *)
-(*   intros. *)
-(*   match goal with *)
-(*   | [ |- ?m = _ ] => canonicalize_map m *)
-(*   end; maps_equal. *)
-(* Qed. *)
-
-(* Definition canon_map {V} (m : NatMap.t V) := *)
-(*   of_list (to_list m). *)
-
-(* Lemma canon_map_ok : *)
-(*   forall {V} (m : NatMap.t V), *)
-(*     m = canon_map m. *)
-(* Proof. *)
-(*   intros. *)
-(*   unfold canon_map. *)
-(*   pose proof (of_list_3 m). *)
-(*   apply map_eq_Equal in H. *)
-(*   rewrite H. *)
-(*   trivial. *)
-(* Qed. *)
-
-(* (* Use if the keys are concrete. Faster and it sorts by key so order is consistent *) *)
-(* Definition canonicalize_concrete_map {v} (m : NatMap.t v) : NatMap.t v. *)
-(*   destruct m. *)
-(*   unfold Raw.t in this0. *)
-(*   let f := constr:(fun (acc : NatMap.t v) (cur : nat * v) => *)
-(*                      let (k, v) := cur *)
-(*                      in acc #+ (k, v)) *)
-(*   in let m' := (eval simpl in (fold_left f this0 #0)) *)
-(*   in apply m'. *)
-(* Defined. *)
-
-(* Ltac canonicalize_concrete_map m := *)
-(*   let m' := (eval simpl in (canonicalize_concrete_map m)) *)
-(*   in replace m with m' in * by maps_equal. *)
-
-(* Section MapPredicates. *)
-(*   Variable V : Type. *)
-(*   Variable P : V -> Prop. *)
-
-(*   Inductive Forall_natmap : NatMap.t V -> Prop := *)
-(*   | Empty_Natmap : Forall_natmap $0 *)
-(*   | Add_Natmap k v (m : NatMap.t V) : *)
-(*       P v *)
-(*       -> Forall_natmap m *)
-(*       -> Forall_natmap ( m $+ (k,v)). *)
-
-(*   Lemma Forall_natmap_forall : *)
-(*     forall m, *)
-(*       Forall_natmap m <-> (forall k v, m $? k = Some v -> P v). *)
-(*   Proof. *)
-(*     split. *)
-(*     - induction 1; intros; solve_simple_maps; eauto. *)
-(*     - induction m using P.map_induction_bis; intros; Equal_eq; eauto. *)
-(*       econstructor; solve_simple_maps; eauto. *)
-
-(*       assert (Forall_natmap m). *)
-(*       eapply IHm; intros. *)
-(*       apply H0 with (k:=k); solve_simple_maps; eauto. *)
-
-(*       econstructor; eauto. *)
-(*       eapply H0 with (k := x); clean_map_lookups; auto. *)
-(*   Qed. *)
-
-(*   Lemma Forall_natmap_in_prop : *)
-(*     forall k v m, *)
-(*       Forall_natmap m *)
-(*       -> m $? k = Some v *)
-(*       -> P v. *)
-(*   Proof. *)
-(*     intros. *)
-(*     rewrite Forall_natmap_forall in H; eauto. *)
-(*   Qed. *)
-
-(*   Lemma Forall_natmap_in_prop_add : *)
-(*     forall k v m, *)
-(*       Forall_natmap (m $+ (k,v)) *)
-(*       -> P v. *)
-(*   Proof. *)
-(*     intros. *)
-(*     eapply Forall_natmap_in_prop with (k:=k); eauto; clean_map_lookups; trivial. *)
-(*   Qed. *)
-
-(*   Lemma Forall_natmap_split : *)
-(*     forall k v m, *)
-(*       Forall_natmap (m $+ (k,v)) *)
-(*       -> ~ In k m *)
-(*       -> Forall_natmap m *)
-(*       /\ P v. *)
-(*   Proof. *)
-(*     intros. *)
-(*     rewrite Forall_natmap_forall in *; intros. *)
-(*     assert (P v) by (eapply H with (k0:=k); clean_map_lookups; trivial). *)
-(*     split; auto; intros. *)
-(*     destruct (k ==n k0); subst; clean_map_lookups; eauto. *)
-(*     eapply H with (k0:=k0); clean_map_lookups; trivial. *)
-(*   Qed. *)
-
-(* End MapPredicates. *)
-
-
-(* Section ConcreteMaps. *)
-
-(*   Definition next_key {V} (m : NatMap.t V) : nat := *)
-(*     match max_elt m with *)
-(*     | None => 0 *)
-(*     | Some (k,v) => S k *)
-(*     end. *)
-
-(*   Lemma max_elt_add_ne_recur : *)
-(*     forall {V} (m : NatMap.t V) k1 k2 v1 v2, *)
-(*       m $? k1 = None *)
-(*       -> k1 <> k2 *)
-(*       -> max_elt (m $+ (k1,v1)) = Some (k2,v2) *)
-(*       -> max_elt m = Some (k2,v2). *)
-(*   Proof. *)
-(*     induction m using map_induction_bis; intros; *)
-(*       Equal_eq; eauto. *)
-
-(*     - unfold max_elt, max_elt_aux in H1; simpl in H1; *)
-(*         clean_map_lookups. *)
-
-(*     - destruct (x ==n k1); clean_map_lookups; eauto. *)
-    
-(*   Admitted. *)
-
-(*   Lemma max_elt_ge_elements : *)
-(*     forall {V} (m : NatMap.t V) k v, *)
-(*       max_elt m = Some (k,v) *)
-(*       -> forall k' v', m $? k' = Some v' *)
-(*                  -> le k' k. *)
-(*   Proof. *)
-(*     induction m using map_induction_bis; intros; *)
-(*       Equal_eq; clean_map_lookups; eauto. *)
-
-(*     destruct (x ==n k'); subst; clean_map_lookups; eauto. *)
-(*     - clear IHm. *)
-(*       generalize (max_elt_Above H0); intros MEA. *)
-(*       specialize (MEA k'). *)
-(*       destruct (k ==n k'); subst; clean_map_lookups; eauto. *)
-(*       apply Nat.lt_le_incl. *)
-(*       apply MEA. *)
-(*       rewrite in_find_iff; unfold not; clean_map_lookups. *)
-      
-(*     - destruct (x ==n k); subst; eauto using max_elt_add_ne_recur. *)
-(*       apply Nat.lt_le_incl. *)
-(*       generalize (max_elt_Above H0); intros MEA. *)
-(*       apply MEA. *)
-(*       rewrite in_find_iff; unfold not; clean_map_lookups. *)
-(*   Qed. *)
-
-
-(*   Lemma next_key_not_in : *)
-(*     forall {V} (m : NatMap.t V) k, *)
-(*       k = next_key m *)
-(*       -> m $? k = None. *)
-(*   Proof. *)
-(*     unfold next_key; intros. *)
-(*     cases (max_elt m); subst. *)
-(*     - destruct p; simpl. *)
-(*       cases (m $? S k); eauto. *)
-(*       exfalso. *)
-
-(*       assert (Above k (m $- k)) by eauto using max_elt_Above. *)
-(*       specialize (H (S k)). *)
-
-(*       assert (In (S k) (m $- k)). *)
-(*       rewrite in_find_iff; unfold not; intros. *)
-(*       rewrite remove_neq_o in H0 by eauto; contra_map_lookup. *)
-(*       specialize (H H0). *)
-(*       SearchAbout (_ < _). *)
-(*       assert (k < S k) by eauto using Nat.lt_succ_diag_r. *)
-(*       assert (S k < S k) by eauto using Nat.lt_trans. *)
-(*       SearchAbout (_ < _). *)
-(*       assert (~ (S k < S k)) by eauto using lt_antirefl. *)
-(*       contradiction. *)
-
-(*     - apply max_elt_Empty in Heq. *)
-(*       apply Empty_eq_empty in Heq; subst. *)
-(*       apply lookup_empty_none. *)
-(*   Qed. *)
